DeBruijnSSA/BinSyntax/Rewrite/Region/Eqv.lean
@@ -2,6 +2,7 @@ import DeBruijnSSA.BinSyntax.Typing.Region
 import DeBruijnSSA.BinSyntax.Rewrite.Region.Cong
 import DeBruijnSSA.BinSyntax.Rewrite.Region.Step
 import DeBruijnSSA.BinSyntax.Rewrite.Region.Uniform
+import DeBruijnSSA.BinSyntax.Rewrite.Region.Setoid
 
 import Discretion.Utils.Quotient
 
@@ -19,157 +20,6 @@ variable [Φ: EffInstSet φ (Ty α) ε] [PartialOrder α] [SemilatticeSup ε] [O
 --   | ⟨n + 2, h⟩ => var ⟨by simp at h; exact h, le_refl _⟩
 
 namespace Region
-
--- TODO: move from EqvGen to UniformGen
-
-instance InS.Setoid (φ) [EffInstSet φ (Ty α) ε] (Γ : Ctx α ε) (L : LCtx α) : Setoid (InS φ Γ L)
-  := EqvGen.Setoid InS.CStep
-
-theorem InS.CStep.eqv_to_region {Γ : Ctx α ε} {L : LCtx α} {r r' : InS φ Γ L}
-  (h : r ≈ r') : EqvGen (Region.CStep (φ := φ) Γ L) r r'
-  := by induction h with
-  | rel _ _ h => exact EqvGen.rel _ _ h
-  | refl => exact EqvGen.refl _
-  | symm _ _ _ I => exact I.symm
-  | trans _ _ _ _ _ Il Ir => exact Il.trans _ _ _ Ir
-
-theorem InS.CStep.of_region {Γ : Ctx α ε} {L : LCtx α} {r r' : InS φ Γ L}
-  (h : EqvGen (Region.CStep (φ := φ) Γ L) r r') : r ≈ r'
-  := CStep.eqv_toIns r.prop r'.prop h
-
-theorem InS.eqv_iff {Γ : Ctx α ε} {L : LCtx α} {r r' : InS φ Γ L}
-  : r ≈ r' ↔ EqvGen (Region.CStep (φ := φ) Γ L) r r'
-  := ⟨CStep.eqv_to_region, CStep.of_region⟩
-
-theorem InS.let1_congr {Γ : Ctx α ε} {L : LCtx α}
-  {r r' : InS φ _ L} (a : Term.InS φ Γ ⟨A, e⟩)
-    : r ≈ r' → InS.let1 a r ≈ InS.let1 a r' := by
-  simp only [eqv_iff]
-  apply Region.CStep.let1_eqv a.prop
-
-theorem InS.let2_congr {Γ : Ctx α ε} {L : LCtx α}
-  {r r' : InS φ _ L} (a : Term.InS φ Γ ⟨Ty.prod A B, e⟩)
-    : r ≈ r' → InS.let2 a r ≈ InS.let2 a r' := by
-  simp only [eqv_iff]
-  apply Region.CStep.let2_eqv a.prop
-
-theorem InS.case_left_congr {Γ : Ctx α ε} {L : LCtx α}
-  {r r' : InS φ _ L} (e : Term.InS φ Γ ⟨Ty.coprod A B, e⟩)
-    : r ≈ r' → (s : _) → InS.case e r s ≈ InS.case e r' s := by
-  simp only [eqv_iff]
-  intro pr s
-  apply Region.CStep.case_left_eqv e.prop pr s.prop
-
-theorem InS.case_right_congr {Γ : Ctx α ε} {L : LCtx α}
-  {s s' : InS φ _ L} (e : Term.InS φ Γ ⟨Ty.coprod A B, e'⟩)
-    : (r : _) → s ≈ s' → InS.case e r s ≈ InS.case e r s' := by
-  simp only [eqv_iff]
-  intro r pr
-  apply Region.CStep.case_right_eqv e.prop r.prop pr
-
-theorem InS.case_congr {Γ : Ctx α ε} {L : LCtx α}
-  {r r' s s' : InS φ _ L} (e : Term.InS φ Γ ⟨Ty.coprod A B, e'⟩)
-  (hr : r ≈ r') (hs : s ≈ s') : InS.case e r s ≈ InS.case e r' s' :=
-  (case_left_congr e hr s).trans _ _ _ (case_right_congr e _ hs)
-
-theorem InS.cfg_entry_congr {Γ : Ctx α ε} {L : LCtx α}
-  {R : LCtx α} {β β' : InS φ Γ (R ++ L)} {G} (pβ : β ≈ β')
-  : InS.cfg R β G ≈ InS.cfg R β' G := by
-  simp only [eqv_iff]
-  apply Region.CStep.cfg_entry_eqv rfl
-  rw [eqv_iff] at pβ
-  exact pβ
-  exact λi => (G i).prop
-
-theorem InS.cfg_block_congr {Γ : Ctx α ε} {L : LCtx α}
-  (R : LCtx α) (β : InS φ Γ (R ++ L)) (G) (i) {g' : InS φ (⟨R.get i, ⊥⟩::Γ) (R ++ L)}
-  (pG : (G i) ≈ g')
-  : InS.cfg R β G ≈ InS.cfg R β (Function.update G i g') := by
-  simp only [eqv_iff, cfg]
-  rw [coe_update]
-  apply Region.CStep.cfg_block_eqv
-  exact β.prop
-  exact (λi => (G i).prop)
-  rw [<-eqv_iff]
-  apply pG
-  rfl
-
-theorem InS.cfg_blocks_partial_congr {Γ : Ctx α ε} {L : LCtx α}
-  (R : LCtx α) (β : InS φ Γ (R ++ L)) {G G'} (pG : G ≈ G') (k : ℕ)
-  : InS.cfg R β G ≈ InS.cfg R β (λi => if i < k then (G' i) else (G i)) := by
-  induction k with
-  | zero => simp only [not_lt_zero', ↓reduceIte]; exact Setoid.refl _
-  | succ k I =>
-    apply Setoid.trans I
-    if h : R.length ≤ k then
-      have h : ∀i : Fin R.length, i < k ↔ i < k + 1 := λi =>
-        ⟨λ_ => Nat.lt_of_lt_of_le i.prop (Nat.le_succ_of_le h),
-         λ_ => Nat.lt_of_lt_of_le i.prop h⟩
-      simp only [h]
-      apply Setoid.refl
-    else
-      have h' :
-        (λi : Fin R.length => if i < k + 1 then (G' i) else (G i))
-        = (Function.update
-          (λi : Fin R.length => if i < k then (G' i) else (G i))
-          ⟨k, Nat.lt_of_not_le h⟩ (G' ⟨k, Nat.lt_of_not_le h⟩))
-        := funext (λi => by
-          split
-          case isTrue h =>
-            cases h with
-            | refl => simp
-            | step h =>
-              have h := Nat.lt_of_succ_le h
-              rw [Function.update_noteq]
-              simp [h]
-              simp only [ne_eq, Fin.ext_iff]
-              exact Nat.ne_of_lt h
-          case isFalse h =>
-            have h := Nat.lt_of_succ_le $ Nat.le_of_not_lt h
-            have h' := Nat.not_lt_of_lt $ h
-            rw [Function.update_noteq]
-            simp [h']
-            simp only [ne_eq, Fin.ext_iff]
-            exact Ne.symm $ Nat.ne_of_lt h)
-      rw [h']
-      apply cfg_block_congr
-      simp [pG ⟨k, Nat.lt_of_not_le h⟩]
-
-theorem InS.cfg_blocks_congr {Γ : Ctx α ε} {L : LCtx α}
-  (R : LCtx α) (β : InS φ Γ (R ++ L)) {G G'} (pG : G ≈ G')
-  : InS.cfg R β G ≈ InS.cfg R β G' := by
-  have h : G' = λi : Fin R.length => if i < R.length then (G' i) else (G i) := by simp
-  rw [h]
-  apply cfg_blocks_partial_congr
-  exact pG
-
-theorem InS.cfg_congr {Γ : Ctx α ε} {L : LCtx α}
-  (R : LCtx α) {β β' : InS φ Γ (R ++ L)} (pβ : β ≈ β') {G G'} (pG : G ≈ G')
-  : InS.cfg R β G ≈ InS.cfg R β' G' := by
-  apply Setoid.trans
-  apply cfg_entry_congr
-  assumption
-  apply cfg_blocks_congr
-  assumption
-
-theorem InS.cfg_congr' {Γ : Ctx α ε} {L : LCtx α}
-  (n : ℕ) (R : LCtx α) (hR : R.length = n)
-  {β β' : InS φ Γ (R ++ L)} (pβ : β ≈ β') {G G'} (pG : G ≈ G')
-  : InS.cfg' n R hR β G ≈ InS.cfg' n R hR β' G' := by
-  cases hR
-  apply cfg_congr <;> assumption
-
-theorem InS.vwk_congr {Γ Δ : Ctx α ε} {L : LCtx α} {r r' : InS φ Δ L}
-  (ρ : Γ.InS Δ) : r ≈ r' → r.vwk ρ ≈ r'.vwk ρ := by
-  simp only [eqv_iff]
-  apply CStep.vwk_eqv
-  exact ρ.prop
-
--- TODO: InS.lwk_congr
-
--- theorem InS.wk_congr {Γ : Ctx α ε} {L : LCtx α} {ρ : ℕ → ℕ}
---   {r r' : InS φ Δ L} (h : r ≈ r') (hρ : Γ.Wkn Δ ρ) : r.vwk ρ hρ ≈ r'.vwk ρ hρ := by
---   induction r with
 
 def Eqv (φ) [EffInstSet φ (Ty α) ε] (Γ : Ctx α ε) (L : LCtx α) := Quotient (InS.Setoid φ Γ L)
 
@@ -215,7 +65,7 @@ theorem Eqv.let2_quot {a : Term.InS φ Γ ⟨Ty.prod A B, e⟩} {r : InS φ (⟨
 def Eqv.case
   (e : Term.InS φ Γ ⟨Ty.coprod A B, e⟩) (r : Eqv φ (⟨A, ⊥⟩::Γ) L) (s : Eqv φ (⟨B, ⊥⟩::Γ) L)
   : Eqv φ Γ L := Quotient.liftOn₂ r s (λr s => InS.q (InS.case e r s))
-    (λ_ _ _ _ h1 h2 => Quotient.sound (InS.case_congr e h1 h2))
+    (λ_ _ _ _ h1 h2 => Quotient.sound (InS.case_congr h1 h2))
 
 @[simp]
 theorem InS.case_q {e : Term.InS φ Γ ⟨Ty.coprod A B, e⟩}
@@ -459,15 +309,6 @@ theorem Eqv.vwk1_lwk {Γ : Ctx α ε} {L K : LCtx α} {ρ : L.InS K}
   : (r.lwk ρ).vwk1 = (r.vwk1 (inserted := inserted)).lwk ρ := by
   induction r using Quotient.inductionOn; simp [InS.vwk1_lwk]
 
-theorem InS.let1_op {Γ : Ctx α ε} {L : LCtx α}
-  {r : InS φ (⟨B, ⊥⟩::Γ) L}
-  (f : φ) (hf : Φ.EFn f A B e)
-  (a : Term.InS φ Γ ⟨A, e⟩)
-    : r.let1 (a.op f hf)
-    ≈ (r.vwk1.let1 ((Term.InS.var 0 (by simp)).op f hf)).let1 a
-  := EqvGen.rel _ _ $ Wf.Cong.rel $
-  TStep.step InS.coe_wf InS.coe_wf (FStep.rw (by constructor))
-
 theorem Eqv.let1_op {Γ : Ctx α ε} {L : LCtx α}
   {r : Eqv φ (⟨B, ⊥⟩::Γ) L}
   (f : φ) (hf : Φ.EFn f A B e)
@@ -479,14 +320,6 @@ theorem Eqv.let1_op {Γ : Ctx α ε} {L : LCtx α}
     apply Eqv.sound
     apply InS.let1_op
 
-theorem InS.let1_let1 {Γ : Ctx α ε} {L : LCtx α} {A B : Ty α}
-  {r : InS φ (⟨B, ⊥⟩::Γ) L}
-  (a : Term.InS φ Γ ⟨A, e⟩) (b : Term.InS φ (⟨A, ⊥⟩::Γ) ⟨B, e⟩)
-    : let1 (a.let1 b) r
-    ≈ (let1 a $ let1 b $ r.vwk1)
-  := EqvGen.rel _ _ $ Wf.Cong.rel $
-  TStep.step InS.coe_wf InS.coe_wf (FStep.rw (by constructor))
-
 theorem Eqv.let1_let1 {Γ : Ctx α ε} {L : LCtx α} {A B : Ty α}
   {r : Eqv φ (⟨B, ⊥⟩::Γ) L}
   (a : Term.InS φ Γ ⟨A, e⟩) (b : Term.InS φ (⟨A, ⊥⟩::Γ) ⟨B, e⟩)
@@ -496,17 +329,6 @@ theorem Eqv.let1_let1 {Γ : Ctx α ε} {L : LCtx α} {A B : Ty α}
     simp only [let1_quot, vwk1_quot]
     apply Eqv.sound
     apply InS.let1_let1
-
-theorem InS.let1_pair {Γ : Ctx α ε} {L : LCtx α} {A B : Ty α} (e' := ⊥)
-  {r : InS φ (⟨Ty.prod A B, ⊥⟩::Γ) L}
-  (a : Term.InS φ Γ ⟨A, e⟩) (b : Term.InS φ Γ ⟨B, e⟩)
-    : r.let1 (a.pair b) ≈ (
-      let1 a $
-      let1 (b.wk ⟨Nat.succ, (by simp)⟩) $
-      let1 ((Term.InS.var 1 (by simp)).pair (e := e') (Term.InS.var 0 (by simp))) $
-      r.vwk1.vwk1)
-  := EqvGen.rel _ _ $ Wf.Cong.rel $
-  TStep.step InS.coe_wf InS.coe_wf (FStep.rw (by constructor))
 
 theorem Eqv.let1_pair {Γ : Ctx α ε} {L : LCtx α} {A B : Ty α} (e' := ⊥)
   {r : Eqv φ (⟨Ty.prod A B, ⊥⟩::Γ) L}
@@ -522,14 +344,6 @@ theorem Eqv.let1_pair {Γ : Ctx α ε} {L : LCtx α} {A B : Ty α} (e' := ⊥)
     apply Eqv.sound
     apply InS.let1_pair
 
-theorem InS.let1_inl {Γ : Ctx α ε} {L : LCtx α} {A B : Ty α} (e' := ⊥)
-  {r : InS φ (⟨A.coprod B, ⊥⟩::Γ) L}
-  (a : Term.InS φ Γ ⟨A, e⟩)
-    : r.let1 a.inl
-    ≈ (r.vwk1.let1 ((Term.InS.var 0 (by simp)).inl (e := e'))).let1 a
-  := EqvGen.rel _ _ $ Wf.Cong.rel $
-  TStep.step InS.coe_wf InS.coe_wf (FStep.rw (by constructor))
-
 theorem Eqv.let1_inl {Γ : Ctx α ε} {L : LCtx α} {A B : Ty α} (e' := ⊥)
   {r : Eqv φ (⟨A.coprod B, ⊥⟩::Γ) L}
   (a : Term.InS φ Γ ⟨A, e⟩)
@@ -541,14 +355,6 @@ theorem Eqv.let1_inl {Γ : Ctx α ε} {L : LCtx α} {A B : Ty α} (e' := ⊥)
     apply Eqv.sound
     apply InS.let1_inl
 
-theorem InS.let1_inr {Γ : Ctx α ε} {L : LCtx α} {A B : Ty α} (e' := ⊥)
-  {r : InS φ (⟨A.coprod B, ⊥⟩::Γ) L}
-  (b : Term.InS φ Γ ⟨B, e⟩)
-    : r.let1 b.inr
-    ≈ (r.vwk1.let1 ((Term.InS.var 0 (by simp)).inr (e := e'))).let1 b
-  := EqvGen.rel _ _ $ Wf.Cong.rel $
-  TStep.step InS.coe_wf InS.coe_wf (FStep.rw (by constructor))
-
 theorem Eqv.let1_inr {Γ : Ctx α ε} {L : LCtx α} {A B : Ty α} (e' := ⊥)
   {r : Eqv φ (⟨A.coprod B, ⊥⟩::Γ) L}
   (b : Term.InS φ Γ ⟨B, e⟩)
@@ -559,16 +365,6 @@ theorem Eqv.let1_inr {Γ : Ctx α ε} {L : LCtx α} {A B : Ty α} (e' := ⊥)
     simp only [let1_quot, vwk1_quot]
     apply Eqv.sound
     apply InS.let1_inr
-
-theorem InS.let1_case_t {Γ : Ctx α ε} {L : LCtx α} {A B : Ty α}
-  {s : InS φ (⟨C, ⊥⟩::Γ) L}
-  (a : Term.InS φ Γ ⟨Ty.coprod A B, e⟩)
-  (l : Term.InS φ (⟨A, ⊥⟩::Γ) ⟨C, e⟩)
-  (r : Term.InS φ (⟨B, ⊥⟩::Γ) ⟨C, e⟩)
-    : let1 (a.case l r) s
-    ≈ case a (let1 l s.vwk1) (let1 r s.vwk1)
-  := EqvGen.rel _ _ $ Wf.Cong.rel $
-  TStep.step InS.coe_wf InS.coe_wf (FStep.rw (by constructor))
 
 theorem Eqv.let1_case_t {Γ : Ctx α ε} {L : LCtx α} {A B : Ty α}
   {s : Eqv φ (⟨C, ⊥⟩::Γ) L}
@@ -582,14 +378,6 @@ theorem Eqv.let1_case_t {Γ : Ctx α ε} {L : LCtx α} {A B : Ty α}
     apply Eqv.sound
     apply InS.let1_case_t
 
-theorem InS.let1_abort {Γ : Ctx α ε} {L : LCtx α} {A : Ty α} (e' := ⊥)
-  {r : InS φ (⟨A, ⊥⟩::Γ) L}
-  (a : Term.InS φ Γ ⟨Ty.empty, e⟩)
-    : r.let1 (a.abort _)
-    ≈ (r.vwk1.let1 ((Term.InS.var 0 (by simp)).abort (e := e') _)).let1 a
-  := EqvGen.rel _ _ $ Wf.Cong.rel $
-  TStep.step InS.coe_wf InS.coe_wf (FStep.rw (by constructor))
-
 theorem Eqv.let1_abort {Γ : Ctx α ε} {L : LCtx α} {A : Ty α} (e' := ⊥)
   {r : Eqv φ (⟨A, ⊥⟩::Γ) L}
   (a : Term.InS φ Γ ⟨Ty.empty, e⟩)
@@ -600,18 +388,6 @@ theorem Eqv.let1_abort {Γ : Ctx α ε} {L : LCtx α} {A : Ty α} (e' := ⊥)
     simp only [let1_quot, vwk1_quot]
     apply Eqv.sound
     apply InS.let1_abort
-
-theorem InS.let2_op {Γ : Ctx α ε} {L : LCtx α}
-  {r : InS φ (⟨C, ⊥⟩::⟨B, ⊥⟩::Γ) L}
-  (f : φ) (hf : Φ.EFn f A (Ty.prod B C) e)
-  (a : Term.InS φ Γ ⟨A, e⟩)
-    : r.let2 (a.op f hf) ≈ (
-      let1 a $
-      let2 ((Term.InS.var 0 (by simp)).op f hf) $
-      r.vwk (ρ := ⟨Nat.liftnWk 2 Nat.succ, by apply Ctx.Wkn.sliftn₂; simp⟩))
-  := sorry
-  -- := EqvGen.rel _ _ $ Wf.Cong.rel $
-  -- TStep.step InS.coe_wf InS.coe_wf (FStep.rw (by constructor))
 
 theorem Eqv.let2_op {Γ : Ctx α ε} {L : LCtx α}
   {r : Eqv φ (⟨C, ⊥⟩::⟨B, ⊥⟩::Γ) L}
@@ -627,17 +403,6 @@ theorem Eqv.let2_op {Γ : Ctx α ε} {L : LCtx α}
     apply Eqv.sound
     apply InS.let2_op
 
-theorem InS.let2_pair {Γ : Ctx α ε} {L : LCtx α} {A B : Ty α}
-  {r : InS φ (⟨B, ⊥⟩::⟨A, ⊥⟩::Γ) L}
-  (a : Term.InS φ Γ ⟨A, e⟩)
-  (b : Term.InS φ Γ ⟨B, e⟩)
-    : r.let2 (a.pair b) ≈ (
-      let1 a $
-      let1 (b.wk ⟨Nat.succ, (by simp)⟩) r)
-  := sorry
-  -- := EqvGen.rel _ _ $ Wf.Cong.rel $
-  -- TStep.step InS.coe_wf InS.coe_wf (FStep.rw (by constructor))
-
 theorem Eqv.let2_pair {Γ : Ctx α ε} {L : LCtx α} {A B : Ty α}
   {r : Eqv φ (⟨B, ⊥⟩::⟨A, ⊥⟩::Γ) L}
   (a : Term.InS φ Γ ⟨A, e⟩)
@@ -652,17 +417,6 @@ theorem Eqv.let2_pair {Γ : Ctx α ε} {L : LCtx α} {A B : Ty α}
     apply Eqv.sound
     apply InS.let2_pair
 
-theorem InS.let2_abort {Γ : Ctx α ε} {L : LCtx α} {A : Ty α} (e' := ⊥)
-  {r : InS φ (⟨B, ⊥⟩::⟨A, ⊥⟩::Γ) L}
-  (a : Term.InS φ Γ ⟨Ty.empty, e⟩)
-    : r.let2 (a.abort _) ≈ (
-      let1 a $
-      let2 ((Term.InS.var 0 (by simp)).abort (e := e') (A.prod B)) $
-      r.vwk ⟨Nat.liftnWk 2 Nat.succ, by apply Ctx.Wkn.sliftn₂; simp⟩)
-    := sorry
-  -- := EqvGen.rel _ _ $ Wf.Cong.rel $
-  -- TStep.step InS.coe_wf InS.coe_wf (FStep.rw (by constructor))
-
 theorem Eqv.let2_abort {Γ : Ctx α ε} {L : LCtx α} {A : Ty α} (e' := ⊥)
   {r : Eqv φ (⟨B, ⊥⟩::⟨A, ⊥⟩::Γ) L}
   (a : Term.InS φ Γ ⟨Ty.empty, e⟩)
@@ -676,15 +430,6 @@ theorem Eqv.let2_abort {Γ : Ctx α ε} {L : LCtx α} {A : Ty α} (e' := ⊥)
     apply Eqv.sound
     apply InS.let2_abort
 
-theorem InS.case_op {Γ : Ctx α ε} {L : LCtx α}
-  (f : φ) (hf : Φ.EFn f A (B.coprod C) e)
-  (a : Term.InS φ Γ ⟨A, e⟩) (r : InS φ (⟨B, ⊥⟩::Γ) L) (s : InS φ (⟨C, ⊥⟩::Γ) L)
-  : r.case (a.op f hf) s ≈
-    (let1 a $ case (Term.InS.op f hf (Term.InS.var 0 (by simp))) r.vwk1 s.vwk1)
-  := sorry
-  -- := EqvGen.rel _ _ $ Wf.Cong.rel $
-  -- TStep.step InS.coe_wf InS.coe_wf (FStep.rw (by constructor))
-
 theorem Eqv.case_op {Γ : Ctx α ε} {L : LCtx α}
   (f : φ) (hf : Φ.EFn f A (B.coprod C) e)
   (a : Term.InS φ Γ ⟨A, e⟩) (r : Eqv φ (⟨B, ⊥⟩::Γ) L) (s : Eqv φ (⟨C, ⊥⟩::Γ) L)
@@ -697,14 +442,6 @@ theorem Eqv.case_op {Γ : Ctx α ε} {L : LCtx α}
       simp only [case_quot, vwk1_quot, let1_quot]
       apply Eqv.sound
       apply InS.case_op
-
-theorem InS.case_abort {Γ : Ctx α ε} {L : LCtx α} (e' := ⊥)
-  (a : Term.InS φ Γ ⟨Ty.empty, e⟩) (r : InS φ (⟨A, ⊥⟩::Γ) L) (s : InS φ (⟨B, ⊥⟩::Γ) L)
-  : r.case (a.abort _) s ≈
-    (let1 a $ case (Term.InS.abort (e := e') (Term.InS.var 0 (by simp)) (A.coprod B)) r.vwk1 s.vwk1)
-  := sorry
-  -- := EqvGen.rel _ _ $ Wf.Cong.rel $
-  -- TStep.step InS.coe_wf InS.coe_wf (FStep.rw (by constructor))
 
 theorem Eqv.case_abort {Γ : Ctx α ε} {L : LCtx α} (e' := ⊥)
   (a : Term.InS φ Γ ⟨Ty.empty, e⟩) (r : Eqv φ (⟨A, ⊥⟩::Γ) L) (s : Eqv φ (⟨B, ⊥⟩::Γ) L)
@@ -747,18 +484,6 @@ theorem Eqv.let1_case {Γ : Ctx α ε} {L : LCtx α}
       apply Eqv.sound
       apply InS.let1_case
 
-theorem InS.let2_case {Γ : Ctx α ε} {L : LCtx α}
-  (a : Term.InS φ Γ ⟨A.prod B, ea⟩)
-  (b : Term.InS φ Γ ⟨C.coprod D, eb⟩)
-  {r : InS φ (⟨C, ⊥⟩::⟨B, ⊥⟩::⟨A, ⊥⟩::Γ) L}
-  (s : InS φ (⟨D, ⊥⟩::⟨B, ⊥⟩::⟨A, ⊥⟩::Γ) L)
-    : (let2 a $ case (b.wk ⟨(· + 2), (by simp)⟩) r s) ≈
-      case b
-        (let2 (a.wk ⟨Nat.succ, (by simp)⟩) (r.vwk ⟨Nat.swap0 2, Ctx.Wkn.swap02⟩))
-        (let2 (a.wk ⟨Nat.succ, (by simp)⟩) (s.vwk ⟨Nat.swap0 2, Ctx.Wkn.swap02⟩))
-  := EqvGen.rel _ _ $ Wf.Cong.rel $
-  TStep.step InS.coe_wf InS.coe_wf (FStep.rw (by constructor))
-
 theorem Eqv.let2_case {Γ : Ctx α ε} {L : LCtx α}
   (a : Term.InS φ Γ ⟨A.prod B, ea⟩)
   (b : Term.InS φ Γ ⟨C.coprod D, eb⟩)
@@ -775,16 +500,6 @@ theorem Eqv.let2_case {Γ : Ctx α ε} {L : LCtx α}
       simp only [case_quot, let2_quot, vwk_quot]
       apply Eqv.sound
       apply InS.let2_case
-
-theorem InS.cfg_br_lt {Γ : Ctx α ε} {L : LCtx α}
-  (ℓ) (a : Term.InS φ Γ ⟨A, ⊥⟩)
-  (R : LCtx α)  (G : (i : Fin R.length) → InS φ (⟨R.get i, ⊥⟩::Γ) (R ++ L))
-  (hℓ : (R ++ L).Trg ℓ A) (hℓ' : ℓ < R.length)
-  : (InS.br ℓ a hℓ).cfg R G
-  ≈ (let1 a $ (G ⟨ℓ, hℓ'⟩).vwk_id (by simp only [Ctx.Wkn.lift_id_iff,
-    Prod.mk_le_mk, le_refl, and_true, Ctx.Wkn.id]; exact List.get_append ℓ hℓ' ▸ hℓ.get)).cfg R G
-  := EqvGen.rel _ _ $ Wf.Cong.rel $
-  TStep.step InS.coe_wf InS.coe_wf (FStep.rw (by constructor))
 
 theorem Eqv.cfg_br_lt {Γ : Ctx α ε} {L : LCtx α}
   (ℓ) (a : Term.InS φ Γ ⟨A, ⊥⟩)
@@ -807,14 +522,6 @@ theorem Eqv.cfg_br_lt {Γ : Ctx α ε} {L : LCtx α}
       simp only [InS.cfg_inner_q, hg, InS.vwk_id_q, InS.let1_q]
       apply Eqv.sound
       apply InS.cfg_br_lt
-
-theorem InS.cfg_let1 {Γ : Ctx α ε} {L : LCtx α}
-  (a : Term.InS φ Γ ⟨A, ea⟩)
-  (R : LCtx α) (β : InS φ (⟨A, ⊥⟩::Γ) (R ++ L))
-  (G : (i : Fin R.length) → InS φ (⟨R.get i, ⊥⟩::Γ) (R ++ L))
-    : (let1 a β).cfg R G ≈ (let1 a $ β.cfg R (λi => (G i).vwk1))
-  := EqvGen.rel _ _ $ Wf.Cong.rel $
-  TStep.step InS.coe_wf InS.coe_wf (FStep.rw (by constructor))
 
 theorem Eqv.cfg_let1 {Γ : Ctx α ε} {L : LCtx α}
   (a : Term.InS φ Γ ⟨A, ea⟩)
@@ -842,14 +549,6 @@ theorem Eqv.cfg_let1 {Γ : Ctx α ε} {L : LCtx α}
       apply Eq.symm
       apply Quotient.forall_of_finChoice_eq hG
 
-theorem InS.cfg_let2 {Γ : Ctx α ε} {L : LCtx α}
-  (a : Term.InS φ Γ ⟨Ty.prod A B, ea⟩)
-  (R : LCtx α) (β : InS φ (⟨B, ⊥⟩::⟨A, ⊥⟩::Γ) (R ++ L))
-  (G : (i : Fin R.length) → InS φ (⟨R.get i, ⊥⟩::Γ) (R ++ L))
-    : (let2 a β).cfg R G ≈ (let2 a $ β.cfg R (λi => (G i).vwk1.vwk1))
-  := EqvGen.rel _ _ $ Wf.Cong.rel $
-  TStep.step InS.coe_wf InS.coe_wf (FStep.rw (by constructor))
-
 theorem Eqv.cfg_let2 {Γ : Ctx α ε} {L : LCtx α}
   (a : Term.InS φ Γ ⟨Ty.prod A B, ea⟩)
   (R : LCtx α) (β : Eqv φ (⟨B, ⊥⟩::⟨A, ⊥⟩::Γ) (R ++ L))
@@ -875,17 +574,6 @@ theorem Eqv.cfg_let2 {Γ : Ctx α ε} {L : LCtx α}
       congr
       apply Eq.symm
       apply Quotient.forall_of_finChoice_eq hG
-
-theorem InS.cfg_case {Γ : Ctx α ε} {L : LCtx α}
-  (e : Term.InS φ Γ ⟨Ty.coprod A B, ea⟩)
-  (R : LCtx α)
-  (r : InS φ (⟨A, ⊥⟩::Γ) (R ++ L))
-  (s : InS φ (⟨B, ⊥⟩::Γ) (R ++ L))
-  (G : (i : Fin R.length) → InS φ (⟨R.get i, ⊥⟩::Γ) (R ++ L))
-    : (InS.case e r s).cfg R G
-    ≈ InS.case e (r.cfg R (λi => (G i).vwk1)) (s.cfg R (λi => (G i).vwk1))
-  := EqvGen.rel _ _ $ Wf.Cong.rel $
-  TStep.step InS.coe_wf InS.coe_wf (FStep.rw (by constructor))
 
 theorem Eqv.cfg_case {Γ : Ctx α ε} {L : LCtx α}
   (e : Term.InS φ Γ ⟨Ty.coprod A B, ea⟩)
@@ -925,44 +613,6 @@ theorem Eqv.cfg_case {Γ : Ctx α ε} {L : LCtx α}
     apply Eq.symm
     apply Quotient.forall_of_finChoice_eq hG
 
-theorem InS.cfg_cfg_eqv_cfg' {Γ : Ctx α ε} {L : LCtx α}
-  (R S : LCtx α) (β : InS φ Γ (R ++ (S ++ L)))
-  (G : (i : Fin R.length) → InS φ (⟨R.get i, ⊥⟩::Γ) (R ++ (S ++ L)))
-  (G' : (i : Fin S.length) → InS φ (⟨S.get i, ⊥⟩::Γ) (S ++ L))
-    : (β.cfg R G).cfg S G'
-    ≈ (β.cast rfl (by rw [List.append_assoc])).cfg'
-      (R.length + S.length) (R ++ S) (by rw [List.length_append])
-      (Fin.addCases
-        (λi => (G i).cast (by
-          simp only [List.get_eq_getElem, Fin.cast, Fin.coe_castAdd]
-          rw [List.getElem_append]
-          -- TODO: put in discretion
-          ) (by rw [List.append_assoc]))
-        (λi => ((G' i).lwk (LCtx.InS.add_left_append (S ++ L) R)).cast (by
-          simp only [List.get_eq_getElem, Fin.cast, Fin.coe_natAdd]
-          -- TODO: put in discretion
-          sorry
-        )
-          (by rw [List.append_assoc])))
-  := EqvGen.rel _ _ $ Wf.Cong.rel $
-  TStep.step InS.coe_wf InS.coe_wf (FStep.rw (by
-    simp only [Set.mem_setOf_eq, coe_cfg, id_eq, coe_cfg', coe_cast]
-    apply Rewrite.cast_trg
-    apply Rewrite.cfg_cfg
-    congr
-    funext i
-    if h : i < R.length then
-      have hi : i = Fin.castAdd S.length ⟨i, h⟩ := rfl
-      rw [hi]
-      simp only [Fin.addCases_left]
-      rfl
-    else
-      let hi := Fin.natAdd_subNat_cast (le_of_not_lt h)
-      rw [<-hi]
-      simp only [Fin.addCases_right]
-      rfl
-    ))
-
 -- theorem Eqv.cfg_eqv_cfg' {Γ : Ctx α ε} {L : LCtx α}
 --   (R S : LCtx α) (β : Eqv φ Γ (R ++ (S ++ L)))
 --   (G : (i : Fin R.length) → Eqv φ (⟨R.get i, ⊥⟩::Γ) (R ++ (S ++ L)))
@@ -976,25 +626,10 @@ theorem InS.cfg_cfg_eqv_cfg' {Γ : Ctx α ε} {L : LCtx α}
 --       )
 --   := sorry
 
-theorem InS.cfg_zero {Γ : Ctx α ε} {L : LCtx α}
-  (β : InS φ Γ L)
-  : β.cfg [] (λi => i.elim0) ≈ β
-  := EqvGen.rel _ _ $ Wf.Cong.rel $
-  TStep.step InS.coe_wf InS.coe_wf (FStep.rw (by constructor))
-
 theorem Eqv.cfg_zero {Γ : Ctx α ε} {L : LCtx α}
   (β : Eqv φ Γ L)
   : β.cfg [] (λi => i.elim0) = β
   := by induction β using Quotient.inductionOn with | h β => exact Eqv.sound $ β.cfg_zero
-
-theorem InS.let2_eta {Γ : Ctx α ε} {L : LCtx α}
-  (a : Term.InS φ Γ ⟨Ty.prod A B, ea⟩)
-  (r : InS φ (⟨A.prod B, ⊥⟩::Γ) L)
-    : (let2 a $
-        let1 ((Term.InS.var 1 ⟨by simp, le_refl _⟩).pair (Term.InS.var 0 (by simp))) r.vwk1.vwk1)
-    ≈ let1 a r
-  := EqvGen.rel _ _ $ Wf.Cong.rel $
-  TStep.step InS.coe_wf InS.coe_wf (FStep.rw (by constructor))
 
 theorem Eqv.let2_eta {Γ : Ctx α ε} {L : LCtx α}
   (a : Term.InS φ Γ ⟨Ty.prod A B, ea⟩)
@@ -1003,16 +638,6 @@ theorem Eqv.let2_eta {Γ : Ctx α ε} {L : LCtx α}
         let1 ((Term.InS.var 1 ⟨by simp, le_refl _⟩).pair (Term.InS.var 0 (by simp))) r.vwk1.vwk1)
     = let1 a r
   := by induction r using Quotient.inductionOn with | h r => exact Eqv.sound $ InS.let2_eta a r
-
-theorem InS.wk_cfg {Γ : Ctx α ε} {L : LCtx α}
-  (R S : LCtx α) (β : InS φ Γ (R ++ L))
-  (G : (i : Fin S.length) → InS φ ((List.get S i, ⊥)::Γ) (R ++ L))
-  (ρ : Fin R.length → Fin S.length)
-  (hρ : LCtx.Wkn (R ++ L) (S ++ L) (Fin.toNatWk ρ))
-  : cfg S (β.lwk ⟨Fin.toNatWk ρ, hρ⟩) (λi => (G i).lwk ⟨Fin.toNatWk ρ, hρ⟩)
-  ≈ cfg R β (λi => (G (ρ i)).vwk_id (Ctx.Wkn.id.toFinWk_id hρ i))
-  := EqvGen.rel _ _ $ Wf.Cong.rel $
-  TStep.step InS.coe_wf InS.coe_wf (FStep.reduce (by constructor))
 
 theorem Eqv.wk_cfg {Γ : Ctx α ε} {L : LCtx α}
   (R S : LCtx α) (β : Eqv φ Γ (R ++ L))
@@ -1034,14 +659,6 @@ theorem Eqv.wk_cfg {Γ : Ctx α ε} {L : LCtx α}
       apply Eqv.sound
       apply InS.wk_cfg
 
-theorem InS.case_inl {Γ : Ctx α ε} {L : LCtx α}
-  (e : Term.InS φ Γ ⟨A, ea⟩)
-  (r : InS φ (⟨A, ⊥⟩::Γ) L)
-  (s : InS φ (⟨B, ⊥⟩::Γ) L)
-    : case e.inl r s ≈ let1 e r
-  := EqvGen.rel _ _ $ Wf.Cong.rel $
-  TStep.step InS.coe_wf InS.coe_wf (FStep.reduce (by constructor))
-
 theorem Eqv.case_inl {Γ : Ctx α ε} {L : LCtx α}
   (e : Term.InS φ Γ ⟨A, ea⟩)
   (r : Eqv φ (⟨A, ⊥⟩::Γ) L)
@@ -1052,14 +669,6 @@ theorem Eqv.case_inl {Γ : Ctx α ε} {L : LCtx α}
   induction s using Quotient.inductionOn
   case _ r s =>
   exact Eqv.sound (InS.case_inl e r s)
-
-theorem InS.case_inr {Γ : Ctx α ε} {L : LCtx α}
-  (e : Term.InS φ Γ ⟨B, ea⟩)
-  (r : InS φ (⟨A, ⊥⟩::Γ) L)
-  (s : InS φ (⟨B, ⊥⟩::Γ) L)
-    : case e.inr r s ≈ let1 e s
-  := EqvGen.rel _ _ $ Wf.Cong.rel $
-  TStep.step InS.coe_wf InS.coe_wf (FStep.reduce (by constructor))
 
 theorem Eqv.case_inr {Γ : Ctx α ε} {L : LCtx α}
   (e : Term.InS φ Γ ⟨B, ea⟩)
@@ -1087,16 +696,6 @@ theorem InS.dead_cfg_left {Γ : Ctx α ε} {L : LCtx α}
 
 -- TODO: Eqv.dead_cfg_left; after Eqv.lwk
 
-theorem InS.let1_beta {Γ : Ctx α ε} {L : LCtx α}
-  (a : Term.InS φ Γ ⟨A, ⊥⟩)
-  (r : InS φ (⟨A, ⊥⟩::Γ) L)
-    : let1 a r ≈ r.vsubst a.subst0
-  := EqvGen.rel _ _ $ Wf.Cong.rel $
-  TStep.step InS.coe_wf InS.coe_wf (by
-    constructor
-    sorry
-  )
-
 theorem Eqv.let1_beta {Γ : Ctx α ε} {L : LCtx α}
   (a : Term.InS φ Γ ⟨A, ⊥⟩)
   (r : Eqv φ (⟨A, ⊥⟩::Γ) L)
@@ -1105,19 +704,11 @@ theorem Eqv.let1_beta {Γ : Ctx α ε} {L : LCtx α}
   induction r using Quotient.inductionOn
   exact Eqv.sound (InS.let1_beta a _)
 
-theorem InS.initial {Γ : Ctx α ε} {L : LCtx α} (hi : Γ.IsInitial) (r r' : InS φ Γ L) : r ≈ r'
-  := EqvGen.rel _ _ $ Wf.Cong.rel (TStep.initial hi r.2 r'.2)
-
 theorem Eqv.initial {Γ : Ctx α ε} {L : LCtx α} (hi : Γ.IsInitial) (r r' : Eqv φ Γ L) : r = r'
   := by
   induction r using Quotient.inductionOn
   induction r' using Quotient.inductionOn
   exact Eqv.sound (InS.initial hi _ _)
-
-theorem InS.terminal {Γ : Ctx α ε} {L : LCtx α}
-  (e e' : Term.InS φ Γ ⟨Ty.unit, ⊥⟩) (r : InS φ (⟨Ty.unit, ⊥⟩::Γ) L)
-  : let1 e r ≈ let1 e' r
-  := EqvGen.rel _ _ $ Wf.Cong.rel (TStep.terminal e.2 e'.2 r.2)
 
 theorem Eqv.terminal {Γ : Ctx α ε} {L : LCtx α}
   (e e' : Term.InS φ Γ ⟨Ty.unit, ⊥⟩) (r : Eqv φ (⟨Ty.unit, ⊥⟩::Γ) L)
