DeBruijnSSA/BinSyntax/Rewrite/Region/Uniform.lean
@@ -1,6 +1,6 @@
-import DeBruijnSSA.BinSyntax.Typing.Region.Basic
-import DeBruijnSSA.BinSyntax.Syntax.Compose.Region
+import DeBruijnSSA.BinSyntax.Typing.Region.Compose
 import DeBruijnSSA.BinSyntax.Syntax.Compose.Term
+import DeBruijnSSA.BinSyntax.Rewrite.Region.Cong
 
 import Discretion.Utils.Quotient
 
@@ -12,18 +12,98 @@ namespace Region
 
 open Term
 
+-- Note: this is a PER over well-formed terms
+
 inductive Uniform (P : Ctx α ε → LCtx α → Region φ → Region φ → Prop)
   : Ctx α ε → LCtx α → Region φ → Region φ → Prop
-  | refl : ∀ x, Uniform P Γ L x x
-  | symm : Uniform P Γ L x y → Uniform P Γ L y x
-  | trans : Uniform P Γ L x y → Uniform P Γ L y z → Uniform P Γ L x z
+  | case_left : e.Wf Γ ⟨Ty.coprod A B, e'⟩ → Uniform P (⟨A, ⊥⟩::Γ) L r r' → s.Wf (⟨B, ⊥⟩::Γ) L
+    → Uniform P Γ L (Region.case e r s) (Region.case e r' s)
+  | case_right : e.Wf Γ ⟨Ty.coprod A B, e'⟩ → r.Wf (⟨A, ⊥⟩::Γ) L → Uniform P (⟨B, ⊥⟩::Γ) L s s'
+    → Uniform P Γ L (Region.case e r s) (Region.case e r s')
+  | let1 : a.Wf Γ ⟨A, e⟩ → Uniform P (⟨A, ⊥⟩::Γ) L r r'
+    → Uniform P Γ L (Region.let1 a r) (Region.let1 a r')
+  | let2 : a.Wf Γ ⟨Ty.prod A B, e⟩ → Uniform P (⟨B, ⊥⟩::⟨A, ⊥⟩::Γ) L r r'
+    → Uniform P Γ L (Region.let2 a r) (Region.let2 a r')
+  | cfg_entry (R : LCtx α) :
+    (hR : R.length = n) →
+    Uniform P Γ (R ++ L) β β' →
+    (∀i : Fin n, (G i).Wf (⟨R.get (i.cast hR.symm), ⊥⟩::Γ) (R ++ L)) →
+    Uniform P Γ L (Region.cfg β n G) (Region.cfg β' n G)
+  | cfg_block (R : LCtx α) :
+    (hR : R.length = n) →
+    β.Wf Γ (R ++ L) →
+    (hG : ∀i : Fin n, (G i).Wf (⟨R.get (i.cast hR.symm), ⊥⟩::Γ) (R ++ L)) →
+    (i : Fin n) →
+    Uniform P (⟨R.get (i.cast hR.symm), ⊥⟩::Γ) (R ++ L) (G i) g' →
+    Uniform P Γ L (Region.cfg β n G) (Region.cfg β n (Function.update G i g'))
   | uniform {e : Term φ} {r s : Region φ}
     : e.Wf (⟨A, ⊥⟩::Γ) (B, ⊥)
-    → r.Wf (⟨B, ⊥⟩::Γ) ((C.coprod B)::L)
+    → r.Wf (⟨B, ⊥⟩::⟨A, ⊥⟩::Γ) ((C.coprod B)::L)
     → s.Wf (⟨A, ⊥⟩::Γ) ((C.coprod A)::L)
     → Uniform P (⟨A, ⊥⟩::Γ)
       ((C.coprod B)::L)
       (r.vsubst e.subst0)
       (s.lsubst (ret (sum Term.nil e)).lsubst0)
-    → Uniform P (⟨A, ⊥⟩::Γ) (C::L) r s
+    → Uniform P (⟨A, ⊥⟩::Γ) (C::L) (r.fixpoint.vsubst e.subst0) s.fixpoint
+  | refl : r.Wf Γ L → Uniform P Γ L r r
   | rel : P Γ L x y → Uniform P Γ L x y
+  | symm : Uniform P Γ L x y → Uniform P Γ L y x
+  | trans : Uniform P Γ L x y → Uniform P Γ L y z → Uniform P Γ L x z
+
+theorem Uniform.wf {P : Ctx α ε → LCtx α → Region φ → Region φ → Prop} {Γ L r r'}
+  (toWf : ∀{Γ L r r'}, P Γ L r r' → r.Wf Γ L ∧ r'.Wf Γ L)
+  (p : (Uniform P Γ L) r r') : r.Wf Γ L ∧ r'.Wf Γ L
+  := by induction p with
+  | case_left de _ ds Ir =>
+    have ⟨dr, dr'⟩ := Ir
+    exact ⟨dr.case de ds, dr'.case de ds⟩
+  | case_right de dr _ Is =>
+    have ⟨ds, ds'⟩ := Is
+    exact ⟨dr.case de ds, dr.case de ds'⟩
+  | let1 de _ Ir =>
+    have ⟨dr, dr'⟩ := Ir
+    exact ⟨dr.let1 de, dr'.let1 de⟩
+  | let2 de _ Ir =>
+    have ⟨dr, dr'⟩ := Ir
+    exact ⟨dr.let2 de, dr'.let2 de⟩
+  | cfg_entry R hR _ dG Iβ =>
+    have ⟨dβ, dβ'⟩ := Iβ
+    exact ⟨dβ.cfg _ R hR dG, dβ'.cfg _ R hR dG⟩
+  | cfg_block R hR dβ dG i _ Ig =>
+    have ⟨_, dg'⟩ := Ig
+    constructor
+    exact dβ.cfg _ R hR dG
+    apply dβ.cfg _ R hR
+    intro k
+    simp only [Function.update, eq_rec_constant, dite_eq_ite]
+    split
+    case isTrue h => exact h ▸ dg'
+    case isFalse h => apply dG
+  | uniform de dr ds => exact ⟨Wf.vsubst de.subst0 dr.fixpoint, ds.fixpoint⟩
+  | refl h => exact ⟨h, h⟩
+  | rel h => exact toWf h
+  | symm _ I => exact I.symm
+  | trans _ _ Il Ir => exact ⟨Il.1, Ir.2⟩
+
+theorem Uniform.left {P : Ctx α ε → LCtx α → Region φ → Region φ → Prop} {Γ L r r'}
+  (toWf : ∀{Γ L r r'}, P Γ L r r' → r.Wf Γ L ∧ r'.Wf Γ L)
+  (p : (Uniform P Γ L) r r') : r.Wf Γ L
+  := (Uniform.wf toWf p).1
+
+theorem Uniform.right {P : Ctx α ε → LCtx α → Region φ → Region φ → Prop} {Γ L r r'}
+  (toWf : ∀{Γ L r r'}, P Γ L r r' → r.Wf Γ L ∧ r'.Wf Γ L)
+  (p : (Uniform P Γ L) r r') : r'.Wf Γ L
+  := (Uniform.wf toWf p).2
+
+theorem Uniform.wf_iff {P : Ctx α ε → LCtx α → Region φ → Region φ → Prop} {Γ L r}
+  (toWf : ∀{Γ L r r'}, P Γ L r r' → r.Wf Γ L ∧ r'.Wf Γ L)
+  : (Uniform P Γ L r r) ↔ r.Wf Γ L := ⟨Uniform.left toWf, Uniform.refl⟩
+
+def Uniform.Setoid (P : Ctx α ε → LCtx α → Region φ → Region φ → Prop) (Γ : Ctx α ε) (L : LCtx α)
+  : Setoid (InS φ Γ L) where
+  r x y := Uniform P Γ L x y
+  iseqv := {
+    refl := λx => Uniform.refl x.prop
+    symm := Uniform.symm
+    trans := Uniform.trans
+  }
