DeBruijnSSA/BinSyntax/Typing/LCtx.lean
@@ -11,27 +11,29 @@ variable [Φ: EffInstSet φ (Ty α) ε] [PartialOrder α] [PartialOrder ε] [Bot
 
 abbrev LCtx (α) := List (Ty α)
 
-structure LCtx.Trg (L : LCtx α) (n : ℕ) (A : Ty α) : Prop where
+namespace LCtx
+
+structure Trg (L : LCtx α) (n : ℕ) (A : Ty α) : Prop where
   length : n < L.length
   getElem : A ≤ L[n]
 
-def LCtx.Trg.get (L : LCtx α) {n A} (h : L.Trg n A) : A ≤ L.get ⟨n, h.length⟩ := h.getElem
+def Trg.get (L : LCtx α) {n A} (h : L.Trg n A) : A ≤ L.get ⟨n, h.length⟩ := h.getElem
 
 instance : Append (LCtx α) := (inferInstance : Append (List (Ty α)))
 
 instance : Membership (Ty α) (LCtx α) := (inferInstance : Membership (Ty α) (List (Ty α)))
 
-def LCtx.IsInitial (L : LCtx α) : Prop := ∀A ∈ L, Ty.IsInitial A
+def IsInitial (L : LCtx α) : Prop := ∀A ∈ L, Ty.IsInitial A
 
 @[simp]
-theorem LCtx.IsInitial.append (L K : LCtx α) : (L ++ K).IsInitial ↔ L.IsInitial ∧ K.IsInitial
+theorem IsInitial.append (L K : LCtx α) : (L ++ K).IsInitial ↔ L.IsInitial ∧ K.IsInitial
   := ⟨
     λh => ⟨λV hV => h V (List.mem_append_left _ hV), λV hV => h V (List.mem_append_right _ hV)⟩,
     λ⟨h, h'⟩ V hV => (List.mem_append.mp hV).elim (h V) (h' V)⟩
 
-def LCtx.take (n : ℕ) (L : LCtx α) : LCtx α := List.take n L
+def take (n : ℕ) (L : LCtx α) : LCtx α := List.take n L
 
-def LCtx.drop (n : ℕ) (L : LCtx α) : LCtx α := List.drop n L
+def drop (n : ℕ) (L : LCtx α) : LCtx α := List.drop n L
 
 def FLCtx (α) := Σn, Fin n → Ty α
 
@@ -39,15 +41,15 @@ def FLCtx (α) := Σn, Fin n → Ty α
 
 variable {L K : LCtx α}
 
-def LCtx.Wkn (L K : LCtx α) (ρ : ℕ → ℕ) : Prop -- TODO: fin argument as defeq?
+def Wkn (L K : LCtx α) (ρ : ℕ → ℕ) : Prop -- TODO: fin argument as defeq?
   := ∀i, (h : i < L.length) → K.Trg (ρ i) L[i]
 
-def LCtx.InS (L K : LCtx α) : Type _ := {ρ : ℕ → ℕ | L.Wkn K ρ}
+def InS (L K : LCtx α) : Type _ := {ρ : ℕ → ℕ | L.Wkn K ρ}
 
-instance LCtx.inSCoe : CoeOut (LCtx.InS L K) (ℕ → ℕ)
+instance inSCoe : CoeOut (InS L K) (ℕ → ℕ)
   := ⟨λt => t.val⟩
 
-instance LCtx.InS.instSetoid : Setoid (LCtx.InS L K) where
+instance InS.instSetoid : Setoid (InS L K) where
   r ρ σ := ∀i, i < L.length → (ρ : ℕ → ℕ) i = (σ : ℕ → ℕ) i
   iseqv := {
     refl := (λ_ _ _ => rfl)
@@ -55,60 +57,88 @@ instance LCtx.InS.instSetoid : Setoid (LCtx.InS L K) where
     trans := (λh h' i hi => (h i hi).trans (h' i hi))
   }
 
-def LCtx.InS.cast {L L' K K' : LCtx α} (hL : L = L') (hK : K = K') (ρ : L.InS K) : L'.InS K'
+def InS.cast {L L' K K' : LCtx α} (hL : L = L') (hK : K = K') (ρ : L.InS K) : L'.InS K'
   := ⟨ρ, hL ▸ hK ▸ ρ.2⟩
 
-theorem LCtx.Wkn.id (L : LCtx α) : L.Wkn L id := λ_ hi => ⟨hi, le_refl _⟩
+theorem Wkn.id (L : LCtx α) : L.Wkn L id := λ_ hi => ⟨hi, le_refl _⟩
 
-def LCtx.InS.id (L : LCtx α) : InS L L := ⟨_root_.id, Wkn.id _⟩
+def InS.id (L : LCtx α) : InS L L := ⟨_root_.id, Wkn.id _⟩
 
-theorem LCtx.Wkn_def (L K : LCtx α) (ρ : ℕ → ℕ) : L.Wkn K ρ ↔
+theorem Wkn_def : L.Wkn K ρ ↔
   ∀i, (h : i < L.length) → K.Trg (ρ i) L[i] := Iff.rfl
 
-theorem LCtx.Wkn_def' (L K : LCtx α) (ρ : ℕ → ℕ) : L.Wkn K ρ ↔
+theorem Wkn_def' : L.Wkn K ρ ↔
   ∀i : Fin L.length, K.Trg (ρ i) L[i] := ⟨λh ⟨i, hi⟩ => h i hi, λh i hi => h ⟨i, hi⟩⟩
 
-theorem LCtx.Wkn_iff (L K : LCtx α) (ρ : ℕ → ℕ) : L.Wkn K ρ ↔ @List.NWkn (Ty α)ᵒᵈ _ K L ρ
+theorem Wkn_iff : L.Wkn K ρ ↔ @List.NWkn (Ty α)ᵒᵈ _ K L ρ
   := ⟨λh i hi => have h' := h i hi; ⟨h'.length, h'.get⟩, λh i hi => have h' := h i hi; ⟨h'.1, h'.2⟩⟩
 
-theorem LCtx.Wkn.step {A : Ty α} (h : L.Wkn K ρ) : Wkn L (A::K) (Nat.stepWk ρ)
-  := (Wkn_iff _ _ _).mpr (((Wkn_iff _ _ _).mp h).step _)
+theorem Wkn.lift {lo hi : Ty α} (h : lo ≤ hi) (hρ : Wkn L K ρ)
+  : Wkn (lo::L) (hi::K) (Nat.liftWk ρ)
+  := Wkn_iff.mpr ((Wkn_iff.mp hρ).lift h)
 
-theorem LCtx.Wkn.liftn_append {L K : LCtx α} {ρ : ℕ → ℕ} (R : LCtx α) (h : L.Wkn K ρ)
+def InS.lift {lo hi : Ty α} (h : lo ≤ hi) (ρ : L.InS K) : InS (lo::L) (hi::K)
+  := ⟨Nat.liftWk ρ, ρ.prop.lift h⟩
+
+theorem Wkn.slift {head : Ty α} (hρ : Wkn L K ρ) : Wkn (head::L) (head::K) (Nat.liftWk ρ)
+  := hρ.lift (le_refl head)
+
+def InS.slift {head : Ty α} (ρ : L.InS K) : InS (head::L) (head::K)
+  := ρ.lift (le_refl head)
+
+theorem Wkn.step {head : Ty α} (h : L.Wkn K ρ) : Wkn L (head::K) (Nat.stepWk ρ)
+  := Wkn_iff.mpr ((Wkn_iff.mp h).step _)
+
+theorem Wkn.liftn_append {L K : LCtx α} {ρ : ℕ → ℕ} (R : LCtx α) (h : L.Wkn K ρ)
   : (R ++ L).Wkn (R ++ K) (Nat.liftnWk R.length ρ) := by
-  rw [LCtx.Wkn_iff]
+  rw [Wkn_iff]
   apply List.NWkn.liftn_append
-  rw [<-LCtx.Wkn_iff]
+  rw [<-Wkn_iff]
   exact h
 
-theorem LCtx.Wkn.comp {L K J : LCtx α} {ρ σ}
+theorem Wkn.comp {L K J : LCtx α} {ρ σ}
   : K.Wkn J ρ → L.Wkn K σ → L.Wkn J (ρ ∘ σ)
   := by
-  simp only [LCtx.Wkn_iff]
+  simp only [Wkn_iff]
   apply List.NWkn.comp
 
-def LCtx.InS.comp {L K J : LCtx α} (ρ : LCtx.InS K J) (σ : LCtx.InS L K) : LCtx.InS L J
+@[simp]
+theorem Wkn.succ {head} {L : LCtx α}
+  : Wkn L (head::L) Nat.succ
+  := step (head := head) (id (L := L))
+
+def InS.wk0 {head : Ty α} {L : LCtx α} : InS L (head::L)
+  := ⟨Nat.succ, Wkn.succ⟩
+
+theorem Wkn.wk1 {head inserted : Ty α} {L : LCtx α}
+  : Wkn (head::L) (head::inserted::L) (Nat.liftWk Nat.succ)
+  := succ.slift
+
+def InS.wk1 {head inserted : Ty α} {L : LCtx α} : InS (head::L) (head::inserted::L)
+  := ⟨Nat.liftWk Nat.succ, Wkn.wk1⟩
+
+def InS.comp {L K J : LCtx α} (ρ : InS K J) (σ : InS L K) : InS L J
   := ⟨(ρ : ℕ → ℕ) ∘ (σ : ℕ → ℕ), ρ.2.comp σ.2⟩
 
 @[simp]
-theorem LCtx.InS.coe_comp {L K J : LCtx α} (ρ : LCtx.InS K J) (σ : LCtx.InS L K)
+theorem InS.coe_comp {L K J : LCtx α} (ρ : InS K J) (σ : InS L K)
   : (ρ.comp σ : ℕ → ℕ) = (ρ : ℕ → ℕ) ∘ (σ : ℕ → ℕ)
   := rfl
 
-theorem LCtx.Wkn.add_left_append (original added : LCtx α)
+theorem Wkn.add_left_append (original added : LCtx α)
   : original.Wkn (added ++ original) (· + added.length)
   := λi hi => ⟨
     by rw [List.length_append]; simp [i.add_comm, hi],
     by rw [List.getElem_append_right] <;> simp [hi]⟩
 
-def LCtx.InS.add_left_append (original added : LCtx α) : InS original (added ++ original)
+def InS.add_left_append (original added : LCtx α) : InS original (added ++ original)
   := ⟨(· + added.length), Wkn.add_left_append original added⟩
 
-theorem LCtx.Trg.wk (h : L.Wkn K ρ) (hK : L.Trg n A) : K.Trg (ρ n) A where
+theorem Trg.wk (h : L.Wkn K ρ) (hK : L.Trg n A) : K.Trg (ρ n) A where
   length := (h n hK.length).1
   getElem := le_trans hK.get (h n hK.length).2
 
-theorem LCtx.Wkn.toFinWk_append {L L' R S : LCtx α} {ρ : Fin R.length → Fin S.length}
+theorem Wkn.toFinWk_append {L L' R S : LCtx α} {ρ : Fin R.length → Fin S.length}
   (hρ : (R ++ L).Wkn (S ++ L') (Fin.toNatWk ρ)) (i : Fin R.length)
   : R[i] ≤ S[ρ i] := by
   have hρ := hρ i (Nat.lt_of_lt_of_le i.prop (by simp));
@@ -116,3 +146,23 @@ theorem LCtx.Wkn.toFinWk_append {L L' R S : LCtx α} {ρ : Fin R.length → Fin 
   have hρ := hρ.getElem
   rw [List.getElem_append _ (by simp)] at hρ
   simp [hρ]
+
+theorem Trg.head (h : A' ≤ A) (L : LCtx α) : Trg (A::L) 0 A' where
+  length := by simp
+  getElem := h
+
+@[simp]
+theorem Trg.head_iff {A A' : Ty α} {L : LCtx α} : Trg (A::L) 0 A' ↔ A' ≤ A
+  := ⟨λh => h.getElem, λh => Trg.head h L⟩
+
+theorem Trg.shead {head} : Trg (head::L) 0 head := Trg.head (le_refl _) L
+
+theorem Trg.step {n} {A : Ty α} (h : L.Trg n A) : Trg (B::L) (n + 1) A
+  := ⟨by simp [h.length], h.getElem⟩
+
+theorem Trg.tail {n} {A : Ty α} (h : Trg (B::L) (n + 1) A) : Trg L n A
+  := ⟨Nat.lt_of_succ_lt_succ h.length, h.getElem⟩
+
+@[simp]
+theorem Trg.step_iff {n} {A : Ty α} {L : LCtx α} : Trg (B::L) (n + 1) A ↔ Trg L n A
+  := ⟨λh => h.tail, λh => h.step⟩
