DeBruijnSSA/BinSyntax/Rewrite.lean
@@ -1,3 +1,3 @@
-import DeBruijnSSA.BinSyntax.Rewrite.Region.Equiv
+import DeBruijnSSA.BinSyntax.Rewrite.Region.Eqv
 import DeBruijnSSA.BinSyntax.Rewrite.Region.Subst
 import DeBruijnSSA.BinSyntax.Rewrite.Region.Categorical
